@prefix qudt: <http://qudt.org/1.1/schema/qudt#> .
@prefix owl: <http://www.w3.org/2002/07/owl#> .
@prefix xsd: <http://www.w3.org/2001/XMLSchema#> .
@prefix skos: <http://www.w3.org/2004/02/skos/core#> .
@prefix rdfs: <http://www.w3.org/2000/01/rdf-schema#> .
@prefix acl: <http://www.w3.org/ns/auth/acl#> .
@prefix geo: <http://www.opengis.net/ont/geosparql#> .
@prefix qb: <http://purl.org/linked-data/cube#> .
@prefix dc: <http://purl.org/dc/elements/1.1/> .
@prefix dcterms: <http://purl.org/dc/terms/> .
@prefix dcat: <http://www.w3.org/ns/dcat#> .
@prefix prov: <http://www.w3.org/ns/prov#> .
@prefix foaf: <http://xmlns.com/foaf/0.1/> .
@prefix void: <http://rdfs.org/ns/void#> .
@prefix org: <http://www.w3.org/ns/org#> .
@prefix gn: <http://www.geonames.org/ontology#> .
@prefix vcard: <http://www.w3.org/2006/vcard/ns#> .
@prefix unit: <http://qudt.org/1.1/vocab/unit#> .
@prefix rdf: <http://www.w3.org/1999/02/22-rdf-syntax-ns#> .
@prefix interval: <http://reference.data.gov.uk/def/intervals/> .
@prefix time: <http://www.w3.org/2006/time#> .
@prefix oa: <http://www.w3.org/ns/oa#> .
@prefix : <http://data.syngenta.org/def/upper/> .
@prefix syu: <http://data.syngenta.org/def/upper/> .
@prefix syu-ttl: <http://data.syngenta.org/def/upper> .

@prefix wgs84: <http://www.w3.org/2003/01/geo/wgs84_pos#> .
@prefix geoWeather: <http://data.syngenta.org/def/geoWeather/> .
@prefix geoWeather-ttl: <http://data.syngenta.org/def/geoWeather/> .
@prefix measure: <http://data.syngenta.org/def/geoWeather/Measure/> .
@prefix observation: <http://data.syngenta.org/def/geoWeather/Observation/> .
@prefix geoPoint: <http://data.syngenta.org/def/geoWeather/GeoPoint/> .
@prefix weatherMetric: <http://data.syngenta.org/def/geoWeather/WeatherMetric/> .
@prefix geoSet: <http://data.syngenta.org/def/geoWeather/GeoSet/> .
@prefix polygon: <http://data.syngenta.org/def/geoWeather/Polygon/> .
@prefix entity: <http://data.syngenta.org/def/entity#> .
@prefix scovo:          <http://purl.org/NET/scovo#> .
@prefix qb:             <http://purl.org/linked-data/cube#> .
@prefix ex:             <http://www.example.com/ns#> .

<http://data.syngenta.org/def/geoWeather/v0.1.0> a owl:Ontology ;
        owl:versionInfo "v2.1.0" ;
        owl:versionIRI <http://data.syngenta.org/def/geoWeather/v0.1.0> ;
	dcterms:created "2017-09-22"^^xsd:date ;
	dcterms:modified "2017-10-01"^^xsd:date ;
  	dcterms:creator [
      			rdf:type :Person ;
			foaf:name "Dean Allemang" ; 
			foaf:mbox "dean.allemang@workingontologist.com" ;
			# syu:hasXRDPrefCode "T800707" ; 
			syu:hasXRDPrefTerm "Allemang, Dean" ;
			],
[
                rdf:type :Person ;
            foaf:name "Kurt Cagle" ; 
            foaf:mbox "kurt.cagle@gmail.com" ;
            # syu:hasXRDPrefCode "T800707" ; 
            syu:hasXRDPrefTerm "Cagle,Kurt" ;
            ]
             ;
  	dc:title "Syngenta geoWeather Ontology" ;
	rdfs:comment "This is an import ontology intended to support geoWeather (geoTroll) content."@en ;
	dcterms:format "text/turtle" ;
	dcterms:isVersionOf geoWeather-ttl: ;
	dcterms:replaces <http://data.syngenta.org/def/upper/0.1.0> ;
#	owl:priorVersion <http://data.syngenta.org/def/upper/v2.0.0> ;
	dcterms:issued "2017-09-22"^^xsd:date ;
	dcterms:identifier <http://data.syngenta.org/def/geoWeather> ;
  	rdfs:seeAlso <http://data.syngenta.org/def/geoWeather-linkset> ;
	.


wgs84:lat_long     rdfs:comment    "A comma-separated representation of a latitude, longitude coordinate." ;
                a               rdf:Property ;
                rdfs:label      "lat/long" .

wgs84:alt          rdfs:comment    "The WGS84 altitude of a SpatialThing (decimal meters \nabove the local reference ellipsoid)." ;
                rdfs:domain     wgs84:SpatialThing ;
                a               rdf:Property ;
                rdfs:label      "altitude" .

wgs84:location     rdfs:range      wgs84:SpatialThing ;
                rdfs:comment    "The relation between something and the point, \n or other geometrical thing in space, where it is.  For example, the realtionship between\n a radio tower and a Point with a given lat and long.\n Or a relationship between a park and its outline as a closed arc of points, or a road and\n its location as a arc (a sequence of points).\n Clearly in practice there will be limit to the accuracy of any such statement, but one would expect\n an accuracy appropriate for the size of the object and uses such as mapping .\n " ;
                a               rdf:Property ;
                rdfs:subPropertyOf
                                foaf:based_near ;
                rdfs:label      "location" .

wgs84:long         rdfs:comment    "The WGS84 longitude of a SpatialThing (decimal degrees)." ;
                rdfs:domain     wgs84:SpatialThing ;
                a               rdf:Property ;
                rdfs:label      "longitude" .

wgs84:Point        rdfs:comment    "A point, typically described using a coordinate system relative to Earth, such as WGS84.\n  " ,
                                " \nUniquely identified by lat/long/alt. i.e.\n\nspaciallyIntersects(P1, P2) :- lat(P1, LAT), long(P1, LONG), alt(P1, ALT),\n  lat(P2, LAT), long(P2, LONG), alt(P2, ALT).\n\nsameThing(P1, P2) :- type(P1, Point), type(P2, Point), spaciallyIntersects(P1, P2).\n  " ;
                a               rdfs:Class ;
                rdfs:subClassOf wgs84:SpatialThing ;
                rdfs:label      "point" .

wgs84:             rdfs:comment    "\nRecent changes to this namespace:\n$Log: wgs84_pos.rdf,v $\nRevision 1.22  2009/04/20 15:00:30  timbl\nRemove the time bits which have been deal with elsewhere eg in iCal.\n\nRevision 1.21  2009/04/20 12:52:47  timbl\ntry again\n\nRevision 1.20  2009/04/20 12:42:11  timbl\nAdd Event (edited ages ago and never checked in), and location (following discussion http://chatlogs.planetrdf.com/swig/2009-04-20#T12-36-09)\n\nRevision 1.19  2009/04/20 12:36:31  timbl\nAdd Event (edited ages ago and never checked in), and location (following discussion http://chatlogs.planetrdf.com/swig/2009-04-20#T12-36-09)\n\nRevision 1.18  2006/02/01 22:01:04  danbri\nClarified that lat and long are decimal degrees, and that alt is decimal metres about local reference ellipsoid\n\nRevision 1.17  2004/02/06 17:38:12  danbri\nFixed a bad commit screwup\n\nRevision 1.15  2003/04/19 11:24:08  danbri\nFixed the typo even more.\n\nRevision 1.14  2003/04/19 11:16:56  danbri\nfixed a typo\n\nRevision 1.13  2003/02/19 22:27:27  connolly\nrelaxed domain constraints on lat/long/alt from Point to SpatialThing\n\nRevision 1.12  2003/01/12 01:41:41  danbri\nTrying local copy of XSLT doc.\n\nRevision 1.11  2003/01/12 01:20:18  danbri\nadded a link to morten's xslt rdfs viewer.\n\nRevision 1.10  2003/01/11 18:56:49  danbri\nRemoved datatype range from lat and long properties, since they would\nhave required each occurance of the property to mention the datatype.\n\nRevision 1.9  2003/01/11 11:41:31  danbri\nAnother typo; repaired rdf:Property to rdf:Property x4\n\nRevision 1.8  2003/01/11 11:05:02  danbri\nAdded an rdfs:range for each lat/long/alt property,\nhttp://www.w3.org/2001/XMLSchema#float\n\nRevision 1.7  2003/01/10 20:25:16  danbri\nLonger rdfs:comment for Point, trying to be Earth-centric and neutral about\ncoordinate system(s) at the same time. Feedback welcomed.\n\nRevision 1.6  2003/01/10 20:18:30  danbri\nAdded CVS log comments into the RDF/XML as an rdfs:comment property of the\nvocabulary. Note that this is not common practice (but seems both harmless\nand potentially useful).\n\n\nrevision 1.5\ndate: 2003/01/10 20:14:31;  author: danbri;  state: Exp;  lines: +16 -5\nUpdated schema:\nAdded a dc:date, added url for more info. Changed the rdfs:label of the\nnamespace from gp to geo. Added a class Point, set as the rdfs:domain of\neach property. Added XML comment on the lat_long property suggesting that\nwe might not need it (based on #rdfig commentary from implementors).\n\nrevision 1.4\ndate: 2003/01/10 20:01:07;  author: danbri;  state: Exp;  lines: +6 -5\nFixed typo; several rdfs:about attributes are now rdf:about. Thanks to MortenF in\n#rdfig for catching this error.\n\nrevision 1.3\ndate: 2003/01/10 11:59:03;  author: danbri;  state: Exp;  lines: +4 -3\nfixed buglet in vocab, added more wgs links\n\nrevision 1.2\ndate: 2003/01/10 11:01:11;  author: danbri;  state: Exp;  lines: +4 -4\nRemoved alt from the as-a-flat-string property, and switched from\nspace separated to comma separated.\n\nrevision 1.1\ndate: 2003/01/10 10:53:23;  author: danbri;  state: Exp;\nbasic geo vocab\n\n" ;
                dc:date         "$Date: 2009/04/20 15:00:30 $" ;
                dc:title        "WGS84 Geo Positioning: an RDF vocabulary" ;
                rdfs:label      "geo" ;
                dc:description  "A vocabulary for representing latitude, longitude and \n altitude information in the WGS84 geodetic reference datum. \n Version $Id: wgs84_pos.rdf,v 1.22 2009/04/20 15:00:30 timbl Exp $. See http://www.w3.org/2003/01/geo/ for more details." .

wgs84:SpatialThing rdfs:comment    "Anything with spatial extent, i.e. size, shape, or position.\n e.g. people, places, bowling balls, as well as abstract areas like cubes.\n" ;
                a               rdfs:Class ;
                rdfs:label      "SpatialThing" .

wgs84:lat          rdfs:comment    "The WGS84 latitude of a SpatialThing (decimal degrees)." ;
                rdfs:domain     wgs84:SpatialThing ;
                a               rdf:Property ;
                rdfs:label      "latitude" .	


####################################################
# Ontology DataCube (QB) 
####################################################


# --- DataSets ---------------------------

qb:DataSet a rdfs:Class, owl:Class;
    rdfs:label "Data set"@en;
    rdfs:comment "Represents a collection of observations, possibly organized into various slices, conforming to some common dimensional structure."@en;
    rdfs:subClassOf qb:Attachable;
    owl:equivalentClass scovo:Dataset;
    rdfs:isDefinedBy <http://purl.org/linked-data/cube>;
    .

# --- Observations ---------------------------

qb:Observation a rdfs:Class, owl:Class;
    rdfs:label "Observation"@en;
    rdfs:comment "A single observation in the cube, may have one or more associated measured values"@en;
    rdfs:subClassOf qb:Attachable;
    owl:equivalentClass scovo:Item;
    rdfs:isDefinedBy <http://purl.org/linked-data/cube>;
    .

qb:dataSet a rdf:Property, owl:ObjectProperty;
    rdfs:label "data set"@en;
    rdfs:comment "indicates the data set of which this observation is a part"@en;
    rdfs:domain qb:Observation;
    rdfs:range qb:DataSet;
    owl:equivalentProperty scovo:dataset;
    rdfs:isDefinedBy <http://purl.org/linked-data/cube>;
    .

qb:observation a rdf:Property, owl:ObjectProperty;
    rdfs:label "observation"@en;
    rdfs:comment "indicates a observation contained within this slice of the data set"@en;
    rdfs:domain qb:ObservationGroup;
    rdfs:range qb:Observation;
    rdfs:isDefinedBy <http://purl.org/linked-data/cube>;
    .

qb:ObservationGroup a rdfs:Class, owl:Class;
    rdfs:label "Observation Group"@en;
    rdfs:comment "A, possibly arbitrary, group of observations."@en;
    rdfs:isDefinedBy <http://purl.org/linked-data/cube>;
    .

qb:observationGroup a rdf:Property, owl:ObjectProperty;
    rdfs:label "observation group"@en;
    rdfs:comment "Indicates a group of observations. The domain of this property is left open so that a group may be attached to different resources and need not be restricted to a single DataSet"@en;
    rdfs:range qb:ObservationGroup;
    rdfs:isDefinedBy <http://purl.org/linked-data/cube>;
    .

# --- Slices ---------------------------

qb:Slice a rdfs:Class, owl:Class;
    rdfs:subClassOf qb:ObservationGroup;
    rdfs:label "Slice"@en;
    rdfs:comment "Denotes a subset of a DataSet defined by fixing a subset of the dimensional values, component properties on the Slice"@en;
    rdfs:subClassOf qb:Attachable;
    rdfs:isDefinedBy <http://purl.org/linked-data/cube>;
    .

qb:slice a rdf:Property, owl:ObjectProperty;
    rdfs:subPropertyOf qb:observationGroup;
    rdfs:label "slice"@en;
    rdfs:comment "Indicates a subset of a DataSet defined by fixing a subset of the dimensional values"@en;
    rdfs:domain qb:DataSet;
    rdfs:range qb:Slice;
    rdfs:isDefinedBy <http://purl.org/linked-data/cube>;
    .

# Removed see http://www.w3.org/2011/gld/track/issues/34
#qb:subSlice a rdf:Property, owl:ObjectProperty;
#    rdfs:label "sub slice"@en;
#    rdfs:comment "Indicates a narrower slice which has additional fixed dimensional values, for example a time-series slice might a subSlice of a slice which spans both time and geographic area"@en;
#    rdfs:domain qb:Slice;
#    rdfs:range qb:Slice;
#    rdfs:isDefinedBy <http://purl.org/linked-data/cube>;
#    .

# --- Dimensions, Attributes, Measures ---------------------------

qb:Attachable a rdfs:Class, owl:Class;
    rdfs:label "Attachable (abstract)"@en;
    rdfs:comment "Abstract superclass for everything that can have attributes and dimensions"@en;
    rdfs:isDefinedBy <http://purl.org/linked-data/cube>;
    .

qb:ComponentProperty a rdfs:Class, owl:Class;
    rdfs:label "Component property (abstract)"@en;
    rdfs:subClassOf rdf:Property;
    rdfs:comment "Abstract super-property of all properties representing dimensions, attributes or measures"@en;
    rdfs:isDefinedBy <http://purl.org/linked-data/cube>;
    .
qb:DimensionProperty a rdfs:Class, owl:Class;
    rdfs:label "Dimension property"@en;
    rdfs:comment "The class of components which represent the dimensions of the cube"@en;
    rdfs:subClassOf qb:ComponentProperty;
    rdfs:subClassOf qb:CodedProperty;
    owl:disjointWith qb:MeasureProperty;
    rdfs:isDefinedBy <http://purl.org/linked-data/cube>;
    .
qb:AttributeProperty a rdfs:Class, owl:Class;
    rdfs:label "Attribute property"@en;
    rdfs:comment "The class of components which represent attributes of observations in the cube, e.g. unit of measurement"@en;
    rdfs:subClassOf qb:ComponentProperty;
    owl:disjointWith qb:MeasureProperty;
    rdfs:isDefinedBy <http://purl.org/linked-data/cube>;
    .
qb:MeasureProperty a rdfs:Class, owl:Class;
    rdfs:label "Measure property"@en;
    rdfs:comment "The class of components which represent the measured value of the phenomenon being observed"@en;
    rdfs:subClassOf qb:ComponentProperty;
    owl:disjointWith qb:AttributeProperty;
    owl:disjointWith qb:DimensionProperty;
    rdfs:isDefinedBy <http://purl.org/linked-data/cube>;
    .
qb:CodedProperty a rdfs:Class, owl:Class;
    rdfs:label "Coded property"@en;
    rdfs:subClassOf qb:ComponentProperty;
    rdfs:comment "Superclass of all coded ComponentProperties"@en;
    rdfs:isDefinedBy <http://purl.org/linked-data/cube>;
    .

# --- Reusable general purpose component properties ---------------------------

qb:measureType a qb:DimensionProperty, rdf:Property;
    rdfs:label "measure type"@en;
    rdfs:comment "Generic measure dimension, the value of this dimension indicates which measure (from the set of measures in the DSD) is being given by the obsValue (or other primary measure)"@en;
    rdfs:range  qb:MeasureProperty;
    rdfs:isDefinedBy <http://purl.org/linked-data/cube>;
    .

# --- Data Structure Definitions ---------------------------

qb:DataStructureDefinition a rdfs:Class, owl:Class;
    rdfs:label "Data structure definition"@en;
    rdfs:comment "Defines the structure of a DataSet or slice"@en;
    rdfs:subClassOf qb:ComponentSet ;
    rdfs:isDefinedBy <http://purl.org/linked-data/cube>;
    .

qb:structure a rdf:Property, owl:ObjectProperty;
    rdfs:label "structure"@en;
    rdfs:comment "indicates the structure to which this data set conforms"@en;
    rdfs:domain qb:DataSet;
    rdfs:range qb:DataStructureDefinition;
    rdfs:isDefinedBy <http://purl.org/linked-data/cube>;
    .


qb:component a rdf:Property, owl:ObjectProperty;
    rdfs:label "component specification"@en;
    rdfs:comment "indicates a component specification which is included in the structure of the dataset"@en;
    rdfs:domain qb:DataStructureDefinition;
    rdfs:range qb:ComponentSpecification;
    rdfs:isDefinedBy <http://purl.org/linked-data/cube>;
    .

# --- Component specifications - for qualifying component use in a DSD ---------------------------

qb:ComponentSpecification a rdfs:Class, owl:Class ;
    rdfs:label "Component specification"@en;
    rdfs:comment """Used to define properties of a component (attribute, dimension etc) which are specific to its usage in a DSD."""@en;
    rdfs:subClassOf qb:ComponentSet ;
    rdfs:isDefinedBy <http://purl.org/linked-data/cube>;
    .

qb:ComponentSet a rdfs:Class, owl:Class;
    rdfs:label "Component set"@en;
    rdfs:comment "Abstract class of things which reference one or more ComponentProperties"@en;
    rdfs:isDefinedBy <http://purl.org/linked-data/cube>;
    .

qb:componentProperty a rdf:Property, owl:ObjectProperty;
    rdfs:label "component"@en;
    rdfs:comment "indicates a ComponentProperty (i.e. attribute/dimension) expected on a DataSet, or a dimension fixed in a SliceKey"@en;
    rdfs:domain qb:ComponentSet;
    rdfs:range qb:ComponentProperty;
    rdfs:isDefinedBy <http://purl.org/linked-data/cube>;
    .

qb:order a rdf:Property, owl:DatatypeProperty;
    rdfs:label "order"@en;
    rdfs:comment """indicates a priority order for the components of sets with this structure, used to guide presentations - lower order numbers come before higher numbers, un-numbered components come last"""@en;
    rdfs:domain qb:ComponentSpecification;
    rdfs:range  xsd:int;
    rdfs:isDefinedBy <http://purl.org/linked-data/cube>;
    .

qb:componentRequired a rdf:Property, owl:DatatypeProperty;
    rdfs:label "component required"@en;
    rdfs:comment """Indicates whether a component property is required (true) or optional (false) in the context of a DSD. Only applicable
    to components correspond to an attribute. Defaults to false (optional)."""@en;
    rdfs:domain qb:ComponentSpecification;
    rdfs:range  xsd:boolean;
    rdfs:isDefinedBy <http://purl.org/linked-data/cube>;
    .

qb:componentAttachment a rdf:Property;
    rdfs:label "component attachment"@en;
    rdfs:comment """Indicates the level at which the component property should be attached, this might an qb:DataSet, qb:Slice or qb:Observation, or a qb:MeasureProperty."""@en;
    rdfs:domain qb:ComponentSpecification;
    rdfs:range  rdfs:Class;
    rdfs:isDefinedBy <http://purl.org/linked-data/cube>;
    .

qb:dimension a rdf:Property, owl:ObjectProperty;
    rdfs:label "dimension"@en;
    rdfs:comment "An alternative to qb:componentProperty which makes explicit that the component is a dimension"@en;
    rdfs:subPropertyOf qb:componentProperty;
    rdfs:range qb:DimensionProperty;
    rdfs:isDefinedBy <http://purl.org/linked-data/cube>;
    .

qb:measure a rdf:Property, owl:ObjectProperty;
    rdfs:label "measure"@en;
    rdfs:comment "An alternative to qb:componentProperty which makes explicit that the component is a measure"@en;
    rdfs:subPropertyOf qb:componentProperty;
    rdfs:range qb:MeasureProperty;
    rdfs:isDefinedBy <http://purl.org/linked-data/cube>;
    .

qb:attribute a rdf:Property, owl:ObjectProperty;
    rdfs:label "attribute"@en;
    rdfs:comment "An alternative to qb:componentProperty which makes explicit that the component is a attribute"@en;
    rdfs:subPropertyOf qb:componentProperty;
    rdfs:range qb:AttributeProperty;
    rdfs:isDefinedBy <http://purl.org/linked-data/cube>;
    .

qb:measureDimension a rdf:Property, owl:ObjectProperty;
    rdfs:label "measure dimension"@en;
    rdfs:comment "An alternative to qb:componentProperty which makes explicit that the component is a measure dimension"@en;
    rdfs:subPropertyOf qb:componentProperty;
    rdfs:range qb:DimensionProperty;
    rdfs:isDefinedBy <http://purl.org/linked-data/cube>;
    .

# --- Slice definitions ---------------------------

qb:SliceKey a rdfs:Class, owl:Class;
    rdfs:label "Slice key"@en;
    rdfs:comment "Denotes a subset of the component properties of a DataSet which are fixed in the corresponding slices"@en;
    rdfs:subClassOf qb:ComponentSet ;
    rdfs:isDefinedBy <http://purl.org/linked-data/cube>;
    .

qb:sliceStructure a rdf:Property, owl:ObjectProperty;
    rdfs:label "slice structure"@en;
    rdfs:comment "indicates the sub-key corresponding to this slice"@en;
    rdfs:domain qb:Slice;
    rdfs:range  qb:SliceKey;
    rdfs:isDefinedBy <http://purl.org/linked-data/cube>;
    .

qb:sliceKey a rdf:Property, owl:ObjectProperty;
    rdfs:label "slice key"@en;
    rdfs:comment "indicates a slice key which is used for slices in this dataset"@en;
    rdfs:domain qb:DataStructureDefinition;
    rdfs:range  qb:SliceKey;
    rdfs:isDefinedBy <http://purl.org/linked-data/cube>;
    .

# --- Concepts ---------------------------

qb:concept a rdf:Property, owl:ObjectProperty;
    rdfs:label "concept"@en;
    rdfs:comment "gives the concept which is being measured or indicated by a ComponentProperty"@en;
    rdfs:domain qb:ComponentProperty;
    rdfs:range skos:Concept;
    rdfs:isDefinedBy <http://purl.org/linked-data/cube>;
    .

qb:codeList a rdf:Property, owl:ObjectProperty;
    rdfs:label "code list"@en;
    rdfs:comment "gives the code list associated with a CodedProperty"@en;
    rdfs:domain qb:CodedProperty;
    rdfs:range  [ owl:unionOf (skos:ConceptScheme skos:Collection qb:HierarchicalCodeList)] ;
    rdfs:isDefinedBy <http://purl.org/linked-data/cube>;
    .

qb:HierarchicalCodeList a rdfs:Class, owl:Class;
#    rdfs:subClassOf qb:CodeList;
    rdfs:label "Hierarchical Code List"@en;
    rdfs:comment "Represents a generalized hierarchy of concepts which can be used for coding. The hierarchy is defined by one or more roots together with a property which relates concepts in the hierarchy to thier child concept .  The same concepts may be members of multiple hierarchies provided that different qb:parentChildProperty values are used for each hierarchy."@en;
    rdfs:isDefinedBy <http://purl.org/linked-data/cube>;
    .

qb:hierarchyRoot a rdf:Property, owl:ObjectProperty;
    rdfs:domain qb:HierarchicalCodeList;
    rdfs:comment   "Specifies a root of the hierarchy. A hierarchy may have multiple roots but must have at least one."@en;
    rdfs:isDefinedBy <http://purl.org/linked-data/cube>;
    .

qb:parentChildProperty a rdf:Property, owl:ObjectProperty;
    rdfs:label "parent-child property"@en;
    rdfs:domain qb:HierarchicalCodeList;
    rdfs:range rdf:Property;
    rdfs:comment   "Specifies a property which relates a parent concept in the hierarchy to a child concept."@en;
    rdfs:isDefinedBy <http://purl.org/linked-data/cube>;
    .

#qb:AggregatableHierarchy
#    rdfs:label "Aggregatable Hierarchy"@en;
#    rdfs:subClassOf qb:HierarchicalCodeList;
#    rdfs:comment "Indicates a hierarchy in which each parent concept is a disjoint union of its child concepts. So that measures such as simple counts may be aggregated up the hierarchy."@en;
#    rdfs:isDefinedBy <http://purl.org/linked-data/cube>;
#    .


####################################################
# Class: DataSet 
####################################################

geoWeather:DataSet 
	a owl:Class;
	rdfs:subClassOf qb:DataSet,geoWeather:Entity;
	rdfs:label "DataSet";
	rdfs:comment "This identifies a set of data as a W3C data cube."@en;
	.

geoWeather:Slice 
	a owl:Class;
	rdfs:subClassOf qb:Slice,geoWeather:Entity;
	rdfs:label "Slice";
	rdfs:comment "This identifies a slice of a data set."@en;
	.

geoWeather:ObservationGroup
	a owl:Class;
	rdfs:subClassOf qb:ObservationGroup,geoWeather:Entity;
	rdfs:label "ObservationGroup";
	rdfs:comment "This corresponds to a DataSet Release in the GeoTroll model."@en;
	.

geoWeather:DataSetRelease
	a owl:Class;
	rdfs:subClassOf qb:ObservationGroup,geoWeather:Entity;
	rdfs:label "DataSetRelease";
	rdfs:comment "This is a synonym for Observation Group, though OG should be the preferred term."@en;
	owl:sameAs geoWeather:ObservationGroup;
	.

geoWeather:Observation
    a owl:Class;
    rdfs:subClassOf qb:Observation,geoWeather:Entity;
    rdfs:label "Observation";
    rdfs:comment "This provides a value for a given time, location, dataset, release and measure. It is an extension of a qb:observation."@en;
    .

geoWeather:ObservationSet
    a owl:Class;
    rdfs:subClassOf geoWeather:Entity;
    rdfs:label "Observation Set";
    rdfs:comment """This is an unordered collection of observations (links) at the same time, location, dataset and releast but over all measures. 
    It can be thought of as an n-dimensional vector of observations. There is no corresponding equivalent in the W3C dataCube spec."""@en;
    .

geoWeather:Measure
    a owl:Class;
    rdfs:subClassOf geoWeather:Entity,qb:Dimension;
    rdfs:label "Measure";
    rdfs:comment """This identifies a specific measurement dimension. It may be decomposed into different aspects, 
    such as maximum value of a temperature on a given day."""@en;
    .

geoWeather:WeatherMetric
    a owl:Class;
    rdfs:subClassOf geoWeather:Entity,qb:Dimension;
    rdfs:label "Measure";
    rdfs:comment """This gives the enumeration of specific metric types."""@en;
    .

measure:type
    a owl:ObjectProperty;
    rdfs:label "Type";
    rdfs:domain geoWeather:Measure;
    rdfs:range geoWeather:MeasureType;
    rdfs:comment """This identifies the specific quality, such as air temperature, being measured."""@en;    
    .

measure:method
    a owl:ObjectProperty;
    rdfs:label "Method";
    rdfs:domain geoWeather:Measure;
    rdfs:range geoWeather:MeasureMethod;
    rdfs:comment """This identifies the specific type of measurements, such as a min or max value, being measured."""@en;    
    .

measure:unit
    a owl:ObjectProperty;
    rdfs:label "Method";
    rdfs:domain geoWeather:Measure;
    rdfs:range geoWeather:Unit;
    rdfs:comment """This identifies the units of the quality being measured."""@en;    
    .


geoWeather:MeasureType
    a owl:Class;
    rdfs:subClassOf geoWeather:Entity,qb:Dimension,skos:ConceptScheme;
    rdfs:label "Measure Type";
    rdfs:comment """This identifies the specific quality being measured, such as air temperature."""@en;
    .

geoWeather:MeasureMethod
    a owl:Class;
    rdfs:subClassOf geoWeather:Entity,skos:ConceptScheme;
    rdfs:label "Measure Method";
    rdfs:comment """This identifies the specific computational (or observation) method for determining the data, such as max, min, average, etc."""@en;
    .

geoWeather:Unit
    a owl:Class;
    rdfs:subClassOf geoWeather:Entity,skos:ConceptScheme;
    rdfs:label "Unit";
    rdfs:comment """This gives the unit identifier as an entity. Typically these will be mapped to the qudt ontologies, but will not inherit directly from them."""@en;
    .


geoWeather:WeatherMetricScheme a skos:ConceptScheme;
    skos:prefLabel "Code list for Weather Metrics - codelist scheme"@en;
    rdfs:label "Code list for Weather Metrics - codelist scheme"@en;
    skos:notation "CL_WeatherMetric";
    skos:note "This  code list provides the weather type."@en;
    skos:definition "This establishes the particular aspect of daily weather being measured." ;
    rdfs:seeAlso geoWeather:WeatherMetricType ;
    skos:hasTopConcept 
        geoWeather:weatherMetric-Cloudcover,
        geoWeather:weatherMetric-Evapotranspiration,
        geoWeather:weatherMetric-GlobalRadiation ,
        geoWeather:weatherMetric-HumidityRel ,
        geoWeather:weatherMetric-PictoCode ,
        geoWeather:weatherMetric-Precip ,
        geoWeather:weatherMetric-PrecipDuration ,
        geoWeather:weatherMetric-PrecipProbability ,
        geoWeather:weatherMetric-PrecipPredictability ,
        geoWeather:weatherMetric-PrecipPredictabilityClass ,
        geoWeather:weatherMetric-ShowerProbability ,
        geoWeather:weatherMetric-SunshineDuration ,
        geoWeather:weatherMetric-TempAir ,
        geoWeather:weatherMetric-ThunderstormProbability ,
        geoWeather:weatherMetric-WindDirection ,
        geoWeather:weatherMetric-WindGust ,
        geoWeather:weatherMetric-WindSpeed ;
    .

geoWeather:WeatherMetricType a rdfs:Class, owl:Class;
	rdfs:subClassOf skos:Concept;
	rdfs:label "Code list for weather-related measurement types - codelist class."@en;
	rdfs:seeAlso geoWeather:WeatherMetricScheme;
	.

 




####################################################
# Class: Entity 
####################################################

geoWeather:Entity 
	a owl:Class;
	rdfs:subClassOf skos:prefLabel;
	rdfs:label "Entity";
	rdfs:comment "This (typically) abstract class provides support for name, code, and description content."@en;
	.

entity:name 
	a rdf:Property,owl:FunctionalProperty;
	rdfs:subClassOf skos:prefLabel;
	rdfs:label "Name";
	rdfs:comment "This provides a user interface friendly interface for the resource. ";
	rdfs:domain geoWeather:Entity;
	rdfs:range xsd:string;
	.

entity:description 
	a rdf:Property,owl:FunctionalProperty;
	rdfs:subClassOf skos:comment;
	rdfs:label "Description";
	rdfs:comment "This provides a general definition of the resource. ";
	rdfs:domain geoWeather:Entity;
	rdfs:range xsd:string;
	.

entity:code 
	a rdf:Property,owl:FunctionalProperty;
	rdfs:subClassOf skos:notation;
	rdfs:label "Code";
	rdfs:comment "This typically will be an abbreviation for the resource type in question. ";
	rdfs:domain geoWeather:Entity;
	rdfs:range xsd:string;
	.

entity:hasSample 
	a rdf:Property,owl:FunctionalProperty;
	rdfs:subClassOf skos:notation;
	rdfs:label "Has Sample";
	rdfs:comment "This provides a turtle-based sample illustrating the use of the class in question.";
	rdfs:domain owl:Class;
	rdfs:range xsd:string;
	.


####################################################
# Class: GeoPoint 
####################################################

geoWeather:GeoPoint 
	a owl:Class;
	rdfs:subClassOf wgs84:SpatialThing;
	rdfs:label "GeoPoint";
	rdfs:comment "A WGS84 based spatial thing using decimal degrees latitude and longitude with altitude given in meters."@en;
	.

geoPoint:name
	a rdf:Property;
	rdfs:subPropertyOf entity:name;
	rdfs:label "name";
	rdfs:comment "The name of the location given by the geoPoint."@en;
	rdfs:domain geoWeather:GeoPoint;
	.

geoPoint:description
	a rdf:Property;
	rdfs:subPropertyOf entity:description;
	rdfs:label "description";
	rdfs:comment "The description of the geoPoint."@en;
	rdfs:domain geoWeather:GeoPoint;
	.

geoPoint:code
	a rdf:Property;
	rdfs:subPropertyOf entity:code;
	rdfs:label "code";
	rdfs:comment "A specific code notation identifying the geoPoint. This could be a mixed lat-long or lat-long-alt string, used primarily for text searches."@en;
	rdfs:domain geoWeather:GeoPoint;
	.


geoPoint:latitude 
	a rdf:Property;
	rdfs:subPropertyOf wgs84:lat;
	rdfs:label "latitude";
	rdfs:comment "The geoWeather latitude, in decimal degrees, based on wgs84."@en;
	rdfs:domain geoWeather:GeoPoint;
	rdfs:range xsd:double;
	owl:sameAs geoPoint:lat;
	.

geoPoint:longitude 
	a rdf:Property;
	rdfs:subPropertyOf wgs84:long;
	rdfs:label "longitude";
	rdfs:comment "The geoWeather longitude, in decimal degrees, based on wgs84."@en;
	rdfs:domain geoWeather:GeoPoint;
	rdfs:range xsd:double;
	owl:sameAs geoPoint:long;
	.

geoPoint:altitude 
	a rdf:Property;
	rdfs:subPropertyOf wgs84:alt;
	rdfs:label "alt";
	rdfs:comment "The geoWeather altitude in meters above the model surface, based on wgs84."@en;
	rdfs:domain geoWeather:GeoPoint;
	rdfs:range xsd:double;
	owl:sameAs geoPoint:alt;
	.

geoPoint:feature
	a rdf:Property,owl:FunctionalProperty;
	rdfs:label "feature";
	rdfs:comment "A link to a geoNames entry. Note that in this case, the wgs84: coordinates can be referenced directly from the feature entry."@en;
	rdfs:domain geoWeather:GeoPoint;
	rdfs:range gn:Feature;
	.

geoWeather:GeoPoint entity:hasSample """
 Sample geoPoint:
 geoPoint:SeattleWA
      a geoWeather:geoPoint;
 	  geoPoint:name "Seattle, WA"@en;
 	  geoPoint:latitude "47.6062"^^xsd:double; 
 	  geoPoint:longitude "-122.3321"^^xsd:double;
 	  geoPoint:altitude "157.886"^^xsd:double;
 	.
""".

####################################################
# Class: GeoSet
####################################################

geoWeather:GeoSet 
	a owl:Class;
	rdfs:subClassOf owl:Collection,geoWeather:geoPoint;
	rdfs:label "GeoSet";
	rdfs:comment "An ordered sequence of geopoints, along with a reference point."@en;
	.

geoSet:name
	a rdf:Property;
	rdfs:subPropertyOf entity:name;
	rdfs:label "name";
	rdfs:comment "The name of the region identified by the geoSet."@en;
	rdfs:domain geoWeather:GeoSet;
	.

geoSet:description
	a rdf:Property;
	rdfs:subPropertyOf entity:description;
	rdfs:label "description";
	rdfs:comment "The description of the geoSet."@en;
	rdfs:domain geoWeather:GeoSet;
	.

geoSet:code
	a rdf:Property;
	rdfs:subPropertyOf entity:code;
	rdfs:label "code";
	rdfs:comment "A specific code notation identifying the geoSet."@en;
	rdfs:domain geoWeather:GeoSet;
	.

geoSet:geoPoints
	a rdf:Property;
	rdfs:label "geoPoints";
	rdfs:comment "The ordered  collection of geoPoints."@en;
	rdfs:domain geoWeather:GeoSet;
	rdfs:range owl:Collection;
	.

geoSet:polygon
	a rdf:Property, owl:ObjectProperty;
	rdfs:label "polygon";
	rdfs:comment "A representation of a polygon as a string. This is an abstract property for inheritance by specific polygon encodings."@en;
	rdfs:domain geoWeather:GeoSet;
	rdfs:range xsd:string;
	.

geoSet:WKBPolygon
    a rdf:Property,owl:ObjectProperty;
    rdfs:subPropertyOf geoSet:polygon;
    rdfs:label "WKB polygon";
    rdfs:comment "A representation of a WKB based polygon as a string."@en;
    rdfs:domain geoWeather:GeoSet;
    rdfs:range xsd:string;
    .

geoSet:WKTPolygon
    a rdf:Property,owl:ObjectProperty;
    rdfs:subPropertyOf geoSet:polygon;
    rdfs:label "WKT polygon";
    rdfs:comment "A representation of a WKT based polygon as a string."@en;
    rdfs:domain geoWeather:GeoSet;
    rdfs:range xsd:string;
    .


geoSet:latitude 
    a rdf:Property;
    rdfs:subPropertyOf wgs84:lat;
    rdfs:label "latitude";
    rdfs:comment "The geoWeather latitude, in decimal degrees, based on wgs84."@en;
    rdfs:domain geoWeather:GeoSet;
    rdfs:range xsd:double;
    owl:sameAs geoSet:lat;
    .

geoSet:longitude 
    a rdf:Property;
    rdfs:subPropertyOf wgs84:long;
    rdfs:label "longitude";
    rdfs:comment "The geoWeather longitude, in decimal degrees, based on wgs84."@en;
    rdfs:domain geoWeather:GeoSet;
    rdfs:range xsd:double;
    owl:sameAs geoSet:long;
    .

geoSet:altitude 
    a rdf:Property;
    rdfs:subPropertyOf wgs84:alt;
    rdfs:label "alt";
    rdfs:comment "The geoWeather altitude in meters above the model surface, based on wgs84."@en;
    rdfs:domain geoWeather:GeoSet;
    rdfs:range xsd:double;
    owl:sameAs geoSet:alt;
    .

geoSet:feature
	a owl:FunctionalProperty;
	rdfs:label "feature";
	rdfs:comment "A link to a geoNames entry. Note that in this case, the wgs84: coordinates can be referenced directly from the feature entry."@en;
	rdfs:domain geoWeather:GeoSet;
	rdfs:range gn:Feature;
	.

geoWeather:GeoSet entity:hasSample """
 Sample geoSet:
 geoSet:WesternHemisphere
    a geoWeather:geoSet;
 	  geoSet:name "Western Hemisphere"@en;
 	  geoSet:geoPoints (
		 [geoPoint:lat "0",  geoPoint:long "0"],
       [geoPoint:lat "0",  geoPoint:long "-180"],
       [geoPoint:lat "90", geoPoint:long "0"],
       [geoPoint:lat "0",  geoPoint:long "0"]
       );
 	.
 	""".

geoWeather:GeoSet entity:hasSample """
 Sample geoSet:
 geoSet:WesternHemisphere
    a geoWeather:geoSet;
      geoSet:name "Western Hemisphere"@en;
      geoSet:WKTPolygon "Polygon("0,0 0,-180 90,0 0,0)";
    .
    """.

geoWeather:Polygon
	a owl:Class;
	rdfs:label "Polygon";
	rdfs:comment "A string representation of a polygon."@en;
	.

polygon:value
	a owl:FunctionalProperty;
	rdfs:label "value";
	rdfs:comment "A string representation of a geoSet in a given representation."@en;
	rdfs:domain geoWeather:GeoSet;
	rdfs:range xsd:string;
	.

polygon:type
	a owl:ObjectProperty;
	rdfs:label "value";
	rdfs:comment "An indicator of geoPolygon types, typically WKB or WKT notation. Note, this may be extended out to a formal class if there are enough representations."@en;
	rdfs:domain geoWeather:GeoSet;
	rdfs:range xsd:string;
	.

geoWeather:Polygon entity:hasSample """
 Sample polygon:
 geoSet:WesternHemisphere
    a geoWeather:geoSet;
 	  geoSet:name "Western Hemisphere"@en;
 	  geoSet:polygon [
		 polygon:value "Polygon("0,0 0,-180 90,0 0,0)";
         polygon:type "WKT"
       ];
 	.
""".

